src/dvspec/dafny/specification/consensus.dfy
@@ -19,8 +19,8 @@ module ConsensusSpec
         all_nodes: set<BLSPubkey>,
         decided_value: Optional<D>,
         honest_nodes_status: map<BLSPubkey, HonestNodeStatus>,
-        ghost honest_nodes_validity_functions: map<BLSPubkey, set<D -> bool>>
-        // ghost honest_nodes: set<BLSPubkey>
+        ghost honest_nodes_validity_functions: map<BLSPubkey, set<D -> bool>>,
+        ghost quorum_made_decision: set<BLSPubkey>
     )    
 
     // Move functions f, quorum, and test_quorum to file commons.dfy
@@ -54,6 +54,7 @@ module ConsensusSpec
         && s.honest_nodes_status.Keys == honest_nodes
         && s.honest_nodes_validity_functions == map[]
         && (forall t | t in s.honest_nodes_status.Values :: t == NOT_DECIDED)
+        && s.quorum_made_decision == {}
     }
 
     predicate Next<D(!new, 0)>(
@@ -102,7 +103,8 @@ module ConsensusSpec
         && (
             forall n | n in h_nodes :: 
                 exists vp: D -> bool | vp in s.honest_nodes_validity_functions[n] :: vp(s.decided_value.safe_get())  
-        )
+        )  
+        && s.quorum_made_decision == h_nodes      
     }
 
     // If n = 5, then f(5) = 1 and quorum(n) = 4.
@@ -111,7 +113,7 @@ module ConsensusSpec
         s: ConsensusInstance
     )
     {
-        exists h_nodes :: is_a_valid_decided_value_according_to_set_of_nodes(s, h_nodes)    
+       exists h_nodes :: is_a_valid_decided_value_according_to_set_of_nodes(s, h_nodes)            
     }
 
     function add_set_of_validity_predicates<D(!new, 0)>(
